Stlc/STLCsol.v
@@ -1,2037 +1,5 @@
 
-(*************************************************************************)
-(** The simply-typed lambda calculus in Coq. *)
-(*************************************************************************)
 
-(** An interactive tutorial on developing programming language metatheory.
-    This file uses the simply-typed lambda calculus (STLC) to demonstrate the
-    locally nameless representation of lambda terms and cofinite
-    quantification in judgments.
-
-    This tutorial concentrates on "how" to formalize STLC; for more details
-    about "why" we use this style of development see the associated lecture
-    slides.
-
-    Tutorial author: Stephanie Weirich, based on prior tutorials by Brian
-    Aydemir and Stephanie Weirich, with help from Aaron Bohannon, Nate Foster,
-    Benjamin Pierce, Jeffrey Vaughan, Dimitrios Vytiniotis, and Steve
-    Zdancewic.  Adapted from code by Arthur Chargu'eraud.
-
-*)
-
-
-(*************************************************************************)
-(** * Contents
-
-    - Syntax of STLC
-    - Substitution
-    - Free variables
-    - Properties about basic operations
-
-    - Open
-    - Local closure
-    - Cofinite quantification
-    - Tactic support
-    - Typing environments
-    - Typing relation
-    - Weakening
-    - Substitution
-    - Values and evaluation
-    - Preservation
-    - Progress
-    - Additional properties
-    - Renaming
-    - Decidability of typechecking
-    - Equivalence of exist fresh and cofinite
-
-  Solutions to exercises are in [STLCsol.v].
-*)
-(*************************************************************************)
-
-
-(** First, we import a number of definitions from the Metatheory library (see
-    Metatheory.v).  The following command makes those definitions available in
-    the rest of this file.  This command will only succeed if you have already
-    run "make" in the toplevel directory to compile the Metatheory library and
-    the tutorial files.
-*)
-
-Require Import Metalib.Metatheory.
-
-(** Next, we import the definitions of the simply-typed lambda calculus. *)
-Require Import Definitions.
-
-(** And some auxiliary lemmas about these definitions. *)
-Require Import Lemmas.
-
-(*************************************************************************)
-(** * Encoding terms in STLC *)
-(*************************************************************************)
-
-(*
-  We start with examples of encodings in STLC.
-
-  For example, we can encode the expression (\x:b. Y x) as below.
-  Because "Y" is free variable in this term, we need to assume an
-  atom for this name.
-*)
-
-Parameter Y : var.
-Definition demo_rep1 := abs typ_base (app (var_f Y) (var_b 0)).
-
-(**
-    Below is another example: the encoding of (\x:b. \y:b. (y x)).
-*)
-
-Definition demo_rep2 := abs typ_base (abs typ_base (app (var_b 0) (var_b 1))).
-
-
-(** Exercise: Uncomment and then complete the definitions of the following
-	 lambda calculus terms using the locally nameless representation.
-
-       "two"     :    \s:b->b. \z:b. s (s z)
-
-       "COMB_K"  :    \x:b. \y:b. x
-
-       "COMB_S"  :    \x:b -> b -> b.\y:b -> b.\z:b. x z (y z)
-
-*)
-
-
-Definition two :=
-  (* SOLUTION *)
-  abs (typ_arrow typ_base typ_base)
-                      (abs typ_base (app (var_b 1) (app (var_b 1) (var_b 0)))).
-
-Definition COMB_K :=
-  (* SOLUTION *)
-	abs typ_base
-    (abs typ_base (var_b 1)).
-
-Definition COMB_S :=
-   (* SOLUTION *)
-   abs (typ_arrow typ_base (typ_arrow typ_base typ_base))
-    (abs (typ_arrow typ_base typ_base)
-      (abs (typ_base)
-        (app (app (var_b 2) (var_b 0)) (app (var_b 1) (var_b 0))))).
-
-(* SCW: move to talk slides *)
-(** There are two important advantages of the locally nameless
-    representation:
-     - Alpha-equivalent terms have a unique representation.
-       We're always working up to alpha-equivalence.
-     - Operations such as free variable substitution and free
-       variable calculation have simple recursive definitions
-       (and therefore are simple to reason about).
-
-    Weighed against these advantages are two drawbacks:
-     - The [exp] datatype admits terms, such as [abs 3], where
-       indices are unbound.
-       A term is called "locally closed" when it contains
-       no unbound indices.
-     - We must define *both* bound variable & free variable
-       substitution and reason about how these operations
-       interact with each other.
-*)
-
-
-(*************************************************************************)
-(** * Substitution *)
-(*************************************************************************)
-
-(** The substitution function replaces a free variable with a term.  For
-    simplicity, we define a notation for free variable substitution that
-    mimics standard mathematical notation.  *)
-
-Notation "[ z ~> u ] e" := (subst_exp u z e) (at level 68).
-
-
-(** To demonstrate how free variable substitution works, we need to
-    reason about var equality.
-*)
-
-Parameter Z : var.
-Check (Y == Z).
-
-(** The decidable var equality function returns a sum. If the two
-    vars are equal, the left branch of the sum is returned, carrying
-    a proof of the proposition that the vars are equal.  If they are
-    not equal, the right branch includes a proof of the disequality.
-
-    The demo below uses three new tactics:
-    - The tactic [simpl] reduces a Coq expression to its normal
-      form.
-    - The tactic [destruct (Y==Y)] considers the two possible
-      results of the equality test.
-    - The tactic [Case] marks cases in the proof script.
-      It takes any string as its argument, and puts that string in
-      the hypothesis list until the case is finished.
-*)
-
-Lemma demo_subst1:
-  [Y ~> var_f Z] (abs typ_base (app (var_b 0) (var_f Y))) = (abs typ_base (app (var_b 0) (var_f Z))).
-Proof.
-  simpl.
-  destruct (Y==Y).
-  - Case "left".
-    auto.
-  - Case "right".
-    destruct n. auto.
-Qed.
-
-(** Take-home Exercise: We can use almost the same proof script as
-    above to state how substitution works in the variable case. Try it
-    on your own.  *)
-
-Lemma subst_eq_var: forall (x : var) u,
-  [x ~> u](var_f x) = u.
-Proof.
-  (* SOLUTION *)
-  intros x u.
-  simpl.
-  destruct (x == x).
-  - Case "left".
-    auto.
-  - Case "right".
-    destruct n. auto.
-Qed.
-
-Lemma subst_neq_var : forall (x y : var) u,
-  y <> x -> [x ~> u](var_f y) = var_f y.
-Proof.
-  (* SOLUTION *)
-  intros x y u.
-  simpl.
-  intro Neq.
-  destruct (y == x).
-  - Case "left".
-    destruct Neq. auto.
-  - Case "right".
-    auto.
-Qed.
-
-Lemma subst_same : forall y e, [y ~> var_f y] e = e.
-Proof.
-  (* SOLUTION *)
-  induction e; simpl; intros; default_simp.
-Qed.
-
-(*************************************************************************)
-(** * Free variables and variable sets *)
-(*************************************************************************)
-
-(** The function [fv] calculates the set of free variables in an expression.
-    *)
-
-(* Demo [fsetdec]
-
-   The tactic [fsetdec] solves a certain class of propositions
-   involving finite sets. See the documentation in [FSetWeakDecide]
-   for a full specification.
-*)
-
-Lemma fsetdec_demo : forall (x : atom) (S : atoms),
-  x `in` (singleton x `union` S).
-Proof.
-  fsetdec.
-Qed.
-
-(** Exercise [subst_exp_fresh_eq] To show the ease of reasoning with these
-    definitions, we will prove a standard result from lambda calculus: if a
-    variable does not appear free in a term, then substituting for it has no
-    effect.
-
-    HINTS: Prove this lemma by induction on [e].
-
-    - You will need to use [simpl] in many cases.  You can [simpl] everything
-      everywhere (including hypotheses) with the pattern [simpl in *].
-
-    - Part of this proof includes a false assumption about free variables.
-      Destructing this hypothesis produces a goal about finite set membership
-      that is solvable by [fsetdec].
-
-    - The [f_equal] tactic converts a goal of the form [f e1 = f e1'] in to
-      one of the form [e1 = e1'], and similarly for [f e1 e2 = f e1' e2'],
-      etc.
-*)
-
-Lemma subst_exp_fresh_eq : forall (x : var) e u,
-  x `notin` fv_exp e -> [x ~> u] e = e.
-Proof.
-  (* SOLUTION *)
-  intros x e u H.
-  induction e.
-  - Case "var_b".
-    auto.
-  - Case "var_f".
-    simpl.
-    destruct (x0 == x).
-    + SCase "x0=x".
-      subst. simpl fv_exp in H. fsetdec.
-    + SCase "x0<>x".
-      auto.
-  - Case "abs".
-    simpl.
-    f_equal.
-    auto.
-  - Case "app".
-    simpl in *.
-    f_equal.
-    auto.
-    auto.
-Qed.
-
-(*************************************************************************)
-(* Exercises                                                             *)
-(*************************************************************************)
-
-(*
-   Step through the proof that free variables are not introduced by substitution.
-
-   This proof actually is very automatable ([simpl in *; auto.] takes care of
-   all but the var_f case), but the explicit proof below demonstrates two
-   parts of the finite set library. These two parts are the tactic
-   [destruct_notin] and the lemma [notin_union], both defined in the module
-   [FSetWeakNotin].
-
-   Before stepping through this proof, you should go to that module to read
-   about those definitions and see what other finite set reasoning is
-   available.
-
-  *)
-Lemma fv_exp_subst_exp_notin : forall x y u e,
-   x `notin` fv_exp e ->
-   x `notin` fv_exp u ->
-   x `notin` fv_exp ([y ~> u]e).
-Proof.
-  intros x y u e Fr1 Fr2.
-  induction e; simpl in *.
-  - Case "var_b".
-    assumption.
-  - Case "var_f".
-    destruct (x0 == y).
-      assumption.
-      simpl. assumption.
-  - Case "abs".
-    apply IHe. assumption.
-  - Case "app".
-    destruct_notin.
-    apply notin_union.
-    apply IHe1.
-    assumption.
-    apply IHe2.
-    assumption.
-Qed.
-
-(* Now prove two other properties of substitution and fv *)
-Lemma subst_exp_fresh_same :
-forall u e x,
-  x `notin` fv_exp e ->
-  x `notin` fv_exp ([x ~> u] e).
-Proof.
- (* SOLUTION *)
-  intros.
-  induction e; simpl in *; auto.
-  - destruct (x0 == x).
-    ++ subst. fsetdec.
-    ++ simpl. auto.
-Qed.
-
-Lemma fv_exp_subst_exp_fresh :
-forall e u x,
-  x `notin` fv_exp e ->
-  fv_exp ([x ~> u] e) [=] fv_exp e.
-Proof.
-  (* SOLUTION *)
-  intros.
-  induction e; simpl in *; auto.
-  - fsetdec.
-  - destruct (x0 == x).
-    ++ subst. fsetdec.
-    ++ simpl. fsetdec.
-  - rewrite IHe1.
-    rewrite IHe2.
-    fsetdec.
-    fsetdec.
-    fsetdec.
-Qed.
-
-(*************************************************************************)
-(*                                                                       *)
-(* Lecture 2                                                             *)
-(*                                                                       *)
-(*************************************************************************)
-
-(*************************************************************************)
-(** * Opening *)
-(*************************************************************************)
-
-
-(** Opening replaces an index with a term.  It corresponds to informal
-    substitution for a bound variable, such as in the rule for beta
-    reduction. Note that only "dangling" indices (those that do not
-    refer to any abstraction) can be opened.
-*)
-
-(** Many common applications of opening replace index zero with an
-    expression or variable.  The following definition provides a
-    convenient shorthand for such uses.  Note that the order of
-    arguments is switched relative to the definition above.  For
-    example, [(open e x)] can be read as "substitute the variable [x]
-    for index [0] in [e]" and "open [e] with the variable [x]."
-    Recall that the coercions above let us write [x] in place of
-    [(var_f x)].
-*)
-
-
-Definition open e u := open_exp_wrt_exp_rec 0 u e.
-
-
-Notation "e ^ x"    := (open_exp_wrt_exp e (var_f x)).
-
-(** This next demo shows the operation of [open].  For example, the
-    locally nameless representation of the term (\y. (\x. (y x)) y) is
-    [abs (app (abs (app 1 0)) 0)].  To look at the body without the
-    outer abstraction, we need to replace the indices that refer to
-    that abstraction with a name.  Therefore, we show that we can open
-    the body of the abs above with Y to produce [app (abs (app Y 0))
-    Y)].
-*)
-
-Lemma demo_open :
-  (app (abs typ_base (app (var_b 1) (var_b 0))) (var_b 0)) ^ Y =
-  (app (abs typ_base (app (var_f Y) (var_b 0))) (var_f Y)).
-Proof.
-  unfold open_exp_wrt_exp.
-  unfold open_exp_wrt_exp_rec.
-  simpl.
-  auto.
-Qed.
-
-(* HINT for demo: To show the equality of the two sides below, use the
-   tactics [unfold], which replaces a definition with its RHS and
-   reduces it to head form, and [simpl], which reduces the term the
-   rest of the way.  Then finish up with [auto].  *)
-
-Ltac simpl_open :=
-  unfold open_exp_wrt_exp; unfold open_exp_wrt_exp_rec; simpl;
-  fold open_exp_wrt_exp_rec; fold open_exp_wrt_exp.
-
-(*************************************************************************)
-(** * Local closure *)
-(*************************************************************************)
-
-(* The local closure judgement classifies terms that have no dangling
-   indices.
-
-   Step through this derivation to see why the term is locally closed.
-*)
-
-Lemma demo_lc :
-  lc_exp (app (abs typ_base (app (var_f Y) (var_b 0))) (var_f Y)).
-Proof.
-  eapply lc_app.
-    eapply lc_abs.
-     intro x. simpl_open.
-     auto.
-    auto.
-Qed.
-
-(*************************************************************************)
-(** More Properties about basic operations *)
-(*************************************************************************)
-
-(** The most important properties about open and lc_exp concern their relationship
-    with the free variable and subst functions. *)
-
-
-Lemma subst_exp_open_exp_wrt_exp :
-forall e3 e1 e2 x1,
-  lc_exp e1 ->
-  [x1 ~> e1] (open e3 e2) = open ([x1 ~> e1] e3) ([x1 ~> e1] e2).
-Proof.
-Admitted.
-
-(** We also define a notation for [open_rec] to make stating some of
-    the properties simpler. However, we don't need to use open_rec
-    outside of this part of the tutorial so we make it a local
-    notation, confined to this section. *)
-(*
-Section BasicOperations.
-Local Notation "{ k ~> u } t" := (open_exp_wrt_exp_rec k u t) (at level 67).
-
-
-
-
-
-Inductive degree : nat -> exp -> Prop :=
-  | degree_var_f : forall n1 x1,
-    degree n1 (var_f x1)
-  | degree_var_b : forall n1 n2,
-    lt n2 n1 ->
-    degree n1 (var_b n2)
-  | degree_abs : forall n1 T1 e1,
-    degree (S n1) e1 ->
-    degree n1 (abs T1 e1)
-  | degree_app : forall n1 e1 e2,
-    degree n1 e1 ->
-    degree n1 e2 ->
-    degree n1 (app e1 e2).
-
-Hint Constructors degree.
-
-(** These define only an upper bound, not a strict upper bound. *)
-
-Lemma degree_S :
-(forall n1 e1,
-  degree n1 e1 ->
-  degree (S n1) e1).
-Proof.
-induction 1; eauto.
-Qed.
-
-Lemma subst_exp_degree :
-(forall e1 e2 x1 n1,
-  degree n1 e1 ->
-  degree n1 e2 ->
-  degree n1 (subst_exp e2 x1 e1)).
-Proof.
-  induction 1; intros; simpl; auto.
-  - destruct (x0 == x1); auto.
-  - econstructor. apply IHdegree. apply degree_S. auto.
-Qed.
-
-
-(*
-Lemma subst_exp_open_exp_wrt_exp :
-forall n e3 e1 e2 x1,
-  degree n e2 ->
-  subst_exp e1 x1 (open_exp_wrt_exp_rec n e3 e2) = open_exp_wrt_exp_rec n (subst_exp e1 x1 e3) (subst_exp e1 x1 e2).
-Proof.
-  induction e2; intros.
-  - simpl.
-    destruct (lt_eq_lt_dec n0 n).
-    destruct s. simpl. auto. auto. simpl. auto.
-  - simpl.
-    destruct (x == x1).
-    subst.
-Admitted.
-*)
-
-Lemma open_exp_wrt_exp_degree : (forall e2 e1, degree 0 e2 -> e2 ^ e1 = e2).
-Proof.
-  induction e2; intros.
-  unfold open_exp_wrt_exp.
-  simpl. inversion H; subst.
-Admitted.
-
-
-(** The first property we would like to show is the analogue to
-    [subst_fresh]: index substitution has no effect for closed terms.
-
-    Here is an initial attempt at the proof.
-*)
-
-
-Lemma open_rec_lc_0 : forall k u e,
-  lc_exp e ->
-  e = {k ~> u} e.
-Proof.
-  intros k u e LC.
-  induction LC.
-  Case "lc_var_f".
-    simpl.
-    auto.
-  Case "lc_abs".
-    simpl.
-    f_equal.
-Admitted.
-
-(** At this point there are two problems.  Our goal is about
-    substitution for index [S k] in term [e], while our induction
-    hypothesis IHLC only tells use about index [k] in term [e ^ x].
-
-    To solve the first problem, we generalize our IH over all [k].
-    That way, when [k] is incremented in the [abs] case, it will still
-    apply.  Below, we use the tactic [generalize dependent] to
-    generalize over [k] before using induction.
-*)
-
-Lemma open_rec_lc_1 : forall k u e,
-  lc_exp e ->
-  e = {k ~> u} e.
-Proof.
-  intros k u e LC.
-  generalize dependent k.
-  induction LC.
-  Case "lc_var_f".
-    simpl. auto.
-  Case "lc_abs".
-    simpl.
-    intro k.
-    f_equal.
-Admitted.
-
-(** At this point we are still stuck because the IH concerns
-    [e ^ x] instead of [e]. The result that we need is that if an
-    index substitution has no effect for an opened term, then it has
-    no effect for the raw term (as long as we are *not* substituting
-    for [0], hence [S k] below).
-<<
-   open e x = {S k ~> u}(open e x)  -> e = {S k ~> u} e
->>
-   In other words, expanding the definition of open:
-<<
-   {0 ~> x}e = {S k ~> u}({0 ~> x} e)  -> e = {S k ~> u} e
->>
-   Of course, to prove this result, we must generalize
-   [0] and [S k] to be any pair of inequal numbers to get a strong
-   enough induction hypothesis for the [abs] case.
- *)
-
-Lemma open_rec_lc_core : forall e j v i u,
-  i <> j ->
-  {j ~> v} e = {i ~> u} ({j ~> v} e) ->
-  e = {i ~> u} e.
-Proof.
-Admitted.
-(*
-  induction e; intros j v i u Neq H; simpl in *.
-  Case "var_b".
-    destruct (j == n);  destruct (i == n).
-      SCase "j = n = i".
-        subst n. destruct Neq. auto.
-      SCase "j = n, i <> n".
-        admit.
-      SCase "j <> n, i = n".
-        subst n. simpl in H.
-        destruct (i == i).
-           SSCase "i=i".
-             auto.
-           SSCase "i<>i".
-             destruct n. auto.
-      SCase "j <> n, i <> n".
-        auto.
-  Case "var_f".
-    auto.
-  Case "abs".
-    f_equal.
-    inversion H.
-    apply  IHe with (j := S j) (u := u) (i := S i) (v := v).
-    auto.
-    auto.
-  Case "app".
-    inversion H.
-    f_equal.
-    eapply IHe1; eauto.
-    eapply IHe2; eauto.
-Qed. *)
-
-(* Take-home Exercise: We've proven the above lemma very explicitly,
-   so that you can step through it slowly to see how it
-   works. However, with automation, it is possible to give a *much*
-   shorter proof. Reprove this lemma on your own to see how compact
-   you can make it. *)
-
-(* SOLUTION *)
-Lemma open_rec_lc_core_automated : forall e j v i u,
-  i <> j ->
-  {j ~> v} e = {i ~> u} ({j ~> v} e) ->
-  e = {i ~> u} e.
-Proof with try solve [eauto | congruence].
-  induction e; intros j v i u Neq H; simpl in *;
-      try solve [inversion H; f_equal; eauto].
-  Case "var_b".
-    destruct (j == n)...
-    destruct (i == n)...
-Admitted.
-
-
-(** With the help of this lemma, we can complete the proof. *)
-
-Lemma open_rec_lc : forall k u e,
-  lc_exp e -> e = {k ~> u} e.
-Proof.
-  intros k u e LC.
-  generalize dependent k.
-  induction LC.
-  Case "lc_var_f".
-    simpl.
-    auto.
-  Case "lc_abs".
-    simpl.
-    intro k.
-    f_equal.
-    unfold open_exp_wrt_exp in *.
-    apply open_rec_lc_core with
-      (i := S k) (j := 0) (u := u) (v := var_f Y).
-    auto.
-    auto.
-  Case "lc_app".
-    intro k.
-    simpl.
-    f_equal.
-    auto.
-    auto.
-Qed.
-
-
-(** Take-home Exercise [subst_open_rec] *)
-
-(** The next lemma demonstrates that free variable substitution
-    distributes over index substitution.
-
-    The proof of this lemma is by straightforward induction over
-    [e1]. When [e1] is a free variable, we need to appeal to
-    [open_rec_lc], proved above.
-*)
-
-Lemma subst_open_rec : forall e1 e2 u (x : var) k,
-  lc_exp u ->
-  [x ~> u] ({k ~> e2} e1) = {k ~> [x ~> u] e2} ([x ~> u] e1).
-Proof.
-Admitted.
-(*  (* SOLUTION *)
-  induction e1; intros e2 u x0 k H; simpl in *; f_equal; auto.
-  Case "var_b".
-    destruct (k == n); auto.
-  Case "var_f".
-    destruct (x == x0); subst; auto.
-    apply open_rec_lc; auto.
-Qed.
-*)
-*)
-
-
-(** *** Exercise [subst_exp_open_exp_wrt_exp_var] *)
-
-(** The lemma above is most often used with [e2] as some fresh
-    variable. Therefore, it simplifies matters to define the following useful
-    corollary.
-
-    HINT: Do not use induction.  Rewrite with [subst_exp_open_exp_wrt_exp] and
-    [subst_neq_var].
-
-*)
-
-Lemma subst_exp_open_exp_wrt_exp_var : forall (x y : var) u e,
-  y <> x ->
-  lc_exp u ->
-  ([x ~> u] e) ^ y = [x ~> u] (e ^ y).
-Proof.
-  (* SOLUTION *)
-  intros x y u e Neq H.
-  rewrite subst_exp_open_exp_wrt_exp with (e2 := var_f y); auto.
-  rewrite subst_neq_var; auto.
-Qed.
-
-(** *** Take-home Exercise [subst_intro] *)
-
-(** This lemma states that opening can be replaced with variable
-    opening and substitution.
-
-    HINT: Prove by induction on [e], first generalizing the
-    argument to [open] by using the [generalize] tactic, e.g.,
-    [generalize 0].
-
-*)
-
-Lemma subst_exp_intro : forall (x : var) u e,
-  x `notin` (fv_exp e) ->
-  open e u = [x ~> u](e ^ x).
-Proof.
-  (* SOLUTION *)
-  intros x u e FV_EXP.
-  unfold open.
-  unfold open_exp_wrt_exp.
-  generalize 0.
-  induction e; intro n0; simpl.
-  Case "var_b".
-    destruct (lt_eq_lt_dec n n0).
-    destruct s. simpl. auto.
-    rewrite subst_eq_var. auto.
-    simpl. auto.
-  Case "var_f".
-    destruct (x0 == x). subst. simpl in FV_EXP. fsetdec. auto.
-  Case "abs".
-    f_equal. simpl in FV_EXP. apply IHe. auto.
-  Case "app".
-    simpl in FV_EXP.
-    f_equal.
-    apply IHe1. auto.
-    apply IHe2. auto.
-Qed.
-
-
-(* End BasicOperations. *)
-
-
-(*************************************************************************)
-(** Quantification in inductive predicates. *)
-(*************************************************************************)
-
-(* In the next example, we will reexamine the definition of
-   [lc_exp] in the [abs] case.
-
-   The lemma [subst_lc] says that local closure is preserved by
-   substitution.  Let's start working through this proof.
-*)
-
-Lemma subst_lc0 : forall (x : var) u e,
-  lc_exp e ->
-  lc_exp u ->
-  lc_exp ([x ~> u] e).
-Proof.
-  intros x u e He Hu.
-  induction He.
-  - Case "lc_var_f".
-    simpl.
-    destruct (x0 == x).
-      auto.
-      auto.
-  - Case "lc_abs".
-    simpl.
-    eapply lc_abs.
-    intros x0.
-    rewrite subst_exp_open_exp_wrt_exp_var.
-    apply H0.
-Admitted.
-
-(** Here we are stuck. We don't know that [x0] is not equal to [x],
-    which is a preconduction for [subst_exp_open_exp_wrt_exp_var].
-
-    The solution is to prove an alternative introduction rule for
-    local closure for abstractions.  In the current rule, we need
-    to show that the body of the abstraction is locally closed,
-    no matter what variable we choose for the binder.
-
-
-<<
-  | lc_abs : forall e,
-      (forall x:var, lc_exp (open e x)) ->
-      lc_exp (abs e)
->>
-
-    An easier to use lemma, requires us to only show that the body
-    of the abstraction is locally closed for a *single* variable.
-    The Lemmas file walks through the proof of this result; for
-    convenience we repeat it below.
-*)
-Lemma lc_abs_exists : forall (x : var) e T,
-      lc_exp (e ^ x) ->
-      lc_exp (abs T e).
-Admitted.
-
-(* With this addition, we can complete the proof of subst_lc. *)
-
-Lemma subst_exp_lc_exp : forall (x : var) u e,
-  lc_exp e ->
-  lc_exp u ->
-  lc_exp ([x ~> u] e).
-Proof.
-  intros x u e He Hu.
-  induction He.
-  - Case "lc_var_f".
-    simpl. default_simp.
-  - Case "lc_abs".
-    simpl.
-    pick fresh x0 for {{x}}.  (* make sure that x0 <> x *)
-    eapply (lc_abs_exists x0).
-    rewrite subst_exp_open_exp_wrt_exp_var; auto.
-  - Case "lc_app".
-    default_simp.
-Qed.
-
-
-
-(*
-    The solution is to change the *definition* of local closure so
-    that we get a different induction principle.  Currently, in the
-    [lc_abs] case, we show that an abstraction is locally closed by
-    showing that the body is locally closed after it has been opened
-    with one particular variable.
-
-<<
-  | lc_abs : forall (x : var) e,
-      x `notin` fv_exp e ->
-      lc_exp (open e x) ->
-      lc_exp (abs e)
->>
-
-    Therefore, our induction hypothesis in this case only applies to
-    that variable. From the hypothesis list in the [lc_abs] case:
-
-      x0 : var,
-      IHHe : lc_exp ([x ~> u]open e x0)
-
-    The problem is that we don't have any assumptions about [x0]. It
-    could very well be equal to [x].
-
-    A stronger induction principle provides an IH that applies to many
-    variables. In that case, we could pick one that is "fresh enough".
-    To do so, we need to revise the above definition of lc_exp and replace
-    the type of lc_abs with this one:
-
-<<
-  | lc_abs_c : forall L e,
-      (forall x:var, x `notin` L -> lc_exp (open e x)) ->
-      lc_exp (abs e)
->>
-
-   This rule says that to show that an abstraction is locally closed,
-   we need to show that the body is closed, after it has been opened by
-   any var [x], *except* those in some set [L]. With this rule, the IH
-   in this proof is now:
-
-     H0 : forall x0 : var, x0 `notin` L -> lc_exp ([x ~> u]open e x0)
-
-   Below, lc_c is the local closure judgment revised to use this new
-   rule in the abs case. We call this "cofinite quantification"
-   because the IH applies to an infinite number of vars [x0], except
-   those in some finite set [L].
-
-   Changing the rule in this way does not change what terms are locally
-   closed.  (For more details about cofinite-quantification see:
-   "Engineering Formal Metatheory", Aydemir, Chargu'eraud, Pierce,
-   Pollack, Weirich. POPL 2008.)
-
-*)
-
-(*
-Inductive lc_c : exp -> Prop :=
-  | lc_var_c : forall (x:var),
-      lc_c x
-  | lc_abs_c : forall (L : atoms) e T,
-      (forall x : var, x `notin` L -> lc_c (open e x)) ->
-      lc_c (abs T e)
-  | lc_app_c : forall e1 e2,
-      lc_c e1 ->
-      lc_c e2 ->
-      lc_c (app e1 e2).
-
-Hint Constructors lc_c.
-
-(* Reintroduce notation for [open_rec] so that we can reprove
-   properties about it and the new version of lc_c. *)
-
-Section CofiniteQuantification.
-Local Notation "{ k ~> u } t" := (open_rec k u t) (at level 67).
-
-(* With this new definition, we can almost use the same proof for
-   [open_rec_lc], we only need one change. We need to add the line
-   [pick fresh x for L.]  immediately before the use of [apply
-   open_rec_lc_core].  This tactic, defined in [Metatheory],
-   introduces a new var [x] that is known not to be in the set [L].
-*)
-
-Lemma open_rec_lc_c : forall k u e,
-  lc_c e ->
-  e = {k ~> u} e.
-Proof.
-  intros k u e LC.
-  generalize dependent k.
-  induction LC.
-  Case "lc_var_f".
-    simpl.
-    auto.
-  Case "lc_abs".
-    simpl.
-    intro k.
-    f_equal.
-    unfold open in *.
-    pick fresh x for L.  (* Note: NEW LINE added *)
-    apply open_rec_lc_core with
-      (i := S k) (j := 0) (u := u) (v := var_f x).
-    auto.
-    auto.
-  Case "lc_app".
-    intro k.
-    simpl.
-    f_equal.
-    auto.
-    auto.
-Qed.
-
-(* Take-home Exercise: The next two lemmas have exactly the same
-   proofs as before. *)
-
-Lemma subst_open_rec_c : forall e1 e2 u (x : var) k,
-  lc_c u ->
-  [x ~> u] ({k ~> e2} e1) = {k ~> [x ~> u] e2} ([x ~> u] e1).
-Proof.
-(* SOLUTION *)
-  induction e1; intros e2 u x0 k H; simpl in *; f_equal; auto.
-  Case "var_b".
-    destruct (k == n); auto.
-  Case "var_f".
-    destruct (x == x0); subst; auto.
-    apply open_rec_lc_c; auto.
-Qed.
-
-Lemma subst_open_var_c : forall (x y : var) u e,
-  y <> x ->
-  lc_c u ->
-  open ([x ~> u] e) y = [x ~> u] (open e y).
-Proof.
-  (* SOLUTION *)
-  intros x y u e Neq H.
-  unfold open.
-  rewrite subst_open_rec_c with (e2 := var_f y); auto.
-  rewrite subst_neq_var; auto.
-Qed.
-
-(* Exercise [subst_lc_c]:
-
-   Once we have changed the definition of lc, we can complete the
-   proof of subst_lc.
-
-    HINT: apply lc_abs_c with cofinite set (L `union` singleton x).
-    This gives us an var x0, and a hypothesis that
-    x0 is fresh for both L and x.
-*)
-
-Lemma subst_lc_c : forall (x : var) u e,
-  lc_c e ->
-  lc_c u ->
-  lc_c ([x ~> u] e).
-Proof.
-  intros x u e He Hu.
-  induction He.
-  Case "lc_var_c".
-   simpl.
-   destruct (x0 == x).
-     auto.
-     auto.
-  Case "lc_abs_c".
-    simpl.
-    (* SOLUTION *)
-    apply lc_abs_c with (L := L `union` singleton x).
-    intros x0 Fr.
-    rewrite subst_open_var_c. auto. auto. auto.
-  Case "lc_app_c".
-     simpl. auto.
-Qed.
-
-End CofiniteQuantification.
-*)
-
-(*************************************************************************)
-(** * Tactic support *)
-(*************************************************************************)
-
-(** When picking a fresh var or applying a rule that uses cofinite
-    quantification, choosing a set of vars to be fresh for can be
-    tedious.  In practice, it is simpler to use a tactic to choose the
-    set to be as large as possible.
-
-    The tactic [gather_atoms] is used to collect together all the
-    atoms in the context.  It relies on an auxiliary tactic,
-    [gather_atoms_with] (from MetatheoryAtom), which maps a function
-    that returns a finite set of atoms over all hypotheses with the
-    appropriate type.
-*)
-
-Ltac gather_atoms ::=
-  let A := gather_atoms_with (fun x : atoms => x) in
-  let B := gather_atoms_with (fun x : atom => singleton x) in
-  let C := gather_atoms_with (fun x : list (var * typ) => dom x) in
-  let D := gather_atoms_with (fun x : exp => fv_exp x) in
-  constr:(A `union` B `union` C `union` D).
-
-(** A number of other, useful tactics are defined by the Metatheory
-    library, and each depends on [gather_atoms].  By redefining
-    [gather_atoms], denoted by the [::=] in its definition below, we
-    automatically update these tactics so that they use the proper
-    notion of "all atoms in the context."
-
-    For example, the tactic [(pick fresh x)] chooses an atom fresh for
-    "everything" in the context.  It is the same as [(pick fresh x for
-    L)], except where [L] has been computed by [gather_atoms].
-
-*)
-
-
-(** *** Example
-
-    The tactic [(pick fresh x and apply H)] applies a rule [H] that is
-    defined using cofinite quantification.  It automatically
-    instantiates the finite set of atoms to exclude using
-    [gather_atoms].
-
-    Below, we reprove [subst_lc_c] using [(pick fresh and apply)].
-    Step through the proof below to see how [(pick fresh and apply)]
-    works.
-*)
-
-(*
-Lemma subst_lc_c_alternate_proof : forall (x : atom) u e,
-  lc_c e ->
-  lc_c u ->
-  lc_c ([x ~> u] e).
-Proof.
-  intros x u e He Hu.
-  induction He.
-  Case "var_f".
-   simpl.
-   destruct (x0 == x).
-     auto.
-     auto.
-  Case "abs".
-    simpl.
-    pick fresh y and apply lc_abs_c.
-    (* Here, take note of the hypothesis [Fr]. *)
-    rewrite subst_open_var_c. auto. auto. auto.
-  Case "app".
-     simpl. auto.
-Qed.
-*)
-
-(*************************************************************************)
-(*                                                                       *)
-(*  Coffee break                                                         *)
-(*                                                                       *)
-(*************************************************************************)
-
-
-(*************************************************************************)
-(** * Typing environments *)
-(*************************************************************************)
-
-(** We represent environments as association lists (lists of pairs of
-    keys and values) whose keys are [atom]s.
-*)
-
-(** For STLC, environments bind [atom]s to [typ]s.  We define an
-    abbreviation [env] for the type of these environments.
-
-    Lists are defined in Coq's standard library, with the constructors
-    [nil] and [cons].  The list library includes the [::] notation
-    for cons as well as standard list operations such as append, map,
-    and fold. The infix operation "++" is list append.
-
-    The Metatheory library extends this reasoning by instantiating the
-    AssocList library to provide support for association lists whose
-    keys are [atom]s.  Everything in this library is polymorphic over
-    the type of objects bound in the environment.  Look in AssocList
-    for additional details about the functions and predicates that we
-    mention below.
-*)
-
-(** Environment equality *)
-
-(** When reasoning about environments, we often need to talk about
-    bindings in the "middle" of an environment. Therefore, it is common
-    for lemmas and definitions to use list append in their statements.
-    Unfortunately, list append is associative, so two Coq expressions may
-    denote the same environment even though they are not equal.
-
-    The tactic [simpl_env] reassociates all concatenations of
-    environments to the right.
-*)
-
-Lemma append_assoc_demo : forall (E0 E1 E2 E3:env),
-  E0 ++ (E1 ++ E2) ++ E3 = E0 ++ E1 ++ E2 ++ E3.
-Proof.
-  intros.
-  auto. (* Does nothing. *)
-  simpl_env.
-  reflexivity.
-Qed.
-
-(** To make environments easy to read, instead of building them from
-    [nil] and [cons], we prefer to build them from the following
-    components:
-      - [nil]: The empty list.
-      - [one]: Lists consisting of exactly one item.
-      - [++]:  List append.
-
-   Furthermore, we introduce compact notation for one (singleton lists):
-   [(x ~ T)] is the same as [one (x, T)].
-*)
-
-(** The simpl_env tactic actually puts lists built from only nil, one
-    and [++] into a "normal form". This process reassociates all appends
-    to the right, removes extraneous nils converts cons to singleton
-    lists with an append.
-*)
-
-Lemma simpl_env_demo : forall (x y:atom) (T1 T2:typ) (E F:env),
-   ((x ~ T1) ++ nil) ++ (y,T2) :: (nil ++ E) ++ F =
-   (x ~ T1) ++ (y ~ T2) ++ E ++ F.
-Proof.
-   intros.
-   (* simpl_env puts the left side into the normal form. *)
-   simpl_env.
-   reflexivity.
-Qed.
-
-(** Note that the [simpl] tactic doesn't produce the "normal form" for
-    environments. It should always be followed up with [simpl_env].
-
-    Furthermore, to convert an environment to any equivalent form
-    other than the normal form (perhaps to apply a lemma) use the
-    tactic [rewrite_env].
-*)
-
-Lemma rewrite_env_demo : forall (x y:atom) (T:typ) P,
-  (forall E, P ((x,T):: E) -> True) ->
-  P (x ~ T) ->
-  True.
-Proof.
-  intros x y T P H.
-  (* apply H. fails here. *)
-  rewrite_env ((x,T) :: nil).
-  apply H.
-Qed.
-
-(** Environment operations. *)
-
-(** The ternary predicate [binds] holds when a given binding is
-    present somewhere in an environment.
-*)
-
-Lemma binds_demo : forall (x:atom) (T:typ) (E F:env),
-  binds x T (E ++ (x ~ T) ++ F).
-Proof.
-  auto.
-Qed.
-
-(** The function [dom] computes the domain of an environment,
-    returning a finite set of [atom]s. Note that we cannot use Coq's
-    equality for finite sets, we must instead use a defined relation
-    [=] for atom set equality.
- *)
-
-Lemma dom_demo : forall (x y : atom) (T : typ),
-  dom (x ~ T) [=] singleton x.
-Proof.
-  auto.
-Qed.
-
-(** The unary predicate [uniq] holds when each atom is bound at most
-    once in an environment.
-*)
-
-Lemma uniq_demo : forall (x y : atom) (T : typ),
-  x <> y -> uniq ((x ~ T) ++ (y ~ T)).
-Proof.
-  auto.
-Qed.
-
-
-(*************************************************************************)
-(** * Typing relation *)
-(*************************************************************************)
-
-(** The definition of the typing relation is straightforward.  In
-    order to ensure that the relation holds for only well-formed
-    environments, we check in the [typing_var] case that the
-    environment is [uniq].  The structure of typing derivations
-    implicitly ensures that the relation holds only for locally closed
-    expressions.
-
-    Finally, note the use of cofinite quantification in
-    the [typing_abs] case.
-*)
-
-Inductive typing_e : env -> exp -> typ -> Prop :=
-  | typing_e_var : forall E (x : atom) T,
-      uniq E ->
-      binds x T E ->
-      typing_e E (var_f x) T
-  | typing_e_abs : forall x E e T1 T2,
-      x `notin` dom E ->
-      typing_e ((x ~ T1) ++ E) (e ^ x) T2 ->
-      typing_e E (abs T1 e) (typ_arrow T1 T2)
-  | typing_e_app : forall E e1 e2 T1 T2,
-      typing_e E e1 (typ_arrow T1 T2) ->
-      typing_e E e2 T1 ->
-      typing_e E (app e1 e2) T2.
-
-(** We add the constructors of the typing relation as hints to be used
-    by the [auto] and [eauto] tactics.
-*)
-
-Hint Constructors typing_e.
-
-
-(*************************************************************************)
-(** * Weakening and CoFinite quantification *)
-(*************************************************************************)
-
-(** Weakening states that if an expression is typeable in some
-    environment, then it is typeable in any well-formed extension of
-    that environment.  This property is needed to prove the
-    substitution lemma.
-
-    As stated below, this lemma is not directly proveable.  The
-    natural way to try proving this lemma proceeds by induction on the
-    typing derivation for [e].
-*)
-
-
-Lemma typing_weakening_0 : forall E F e T,
-  typing_e E e T ->
-  uniq (F ++ E) ->
-  typing_e (F ++ E) e T.
-Proof.
-  intros E F e T H J.
-  induction H; auto.
-  Case "typing_abs".
-    apply (typing_e_abs x).
-    (* ... stuck here ... *)
-Admitted.
-
-(** We are stuck in the [typing_abs] case because the induction
-    hypothesis [IHtyping_e] applies only when we weaken the environment at its
-    head.  In this case, however, we need to weaken the environment in
-    the middle; compare the conclusion at the point where we're stuck
-    to the hypothesis [H], which comes from the given typing derivation.
-
-    We can obtain a more useful induction hypothesis by changing the
-    statement to insert new bindings into the middle of the
-    environment, instead of at the head.  However, the proof still
-    gets stuck, as can be seen by examining each of the cases in
-    the proof below.
-
-    Note: To view subgoal n in a proof, use the command "[Show n]".
-    To work on subgoal n instead of the first one, use the command
-    "[Focus n]".
-*)
-
-Lemma typing_weakening_strengthened_0 : forall (E F G : env) e T,
-  typing_e (G ++ E) e T ->
-  uniq (G ++ F ++ E) ->
-  typing_e (G ++ F ++ E) e T.
-Proof.
-  intros E F G e T H J.
-  induction H.
-  Case "typing_var".
-    (* The G0 looks strange in the [typing_var] case. *)
-  Focus 2.
-  Case "typing_abs".
-    (* The [typing_abs] case still does not have a strong enough IH. *)
-Admitted.
-
-(** The hypotheses in the [typing_var] case include an environment
-    [G0] that that has no relation to what we need to prove.  The
-    missing fact we need is that [G0 = (G ++ E)].
-
-    The problem here arises from the fact that Coq's [induction]
-    tactic let's us only prove something about all typing derivations.
-    While it's clear to us that weakening applies to all typing
-    derivations, it's not clear to Coq, because the environment is
-    written using concatenation.  The [induction] tactic expects that
-    all arguments to a judgement are variables.  So we see [E0] in the
-    proof instead of [(G ++ E)].
-
-    The solution is to restate the lemma.  For example, we can prove
-
-<<
-  forall E F E' e T, typing E' e T ->
-  forall G, E' = G ++ E -> uniq (G ++ F ++ E) -> typing (G ++ F ++ E) e T.
->>
-
-    The equality gets around the problem with Coq's [induction]
-    tactic.  The placement of the [(forall G)] quantifier gives us a
-    sufficiently strong induction hypothesis in the [typing_abs] case.
-
-    However, we prefer not to state the lemma in the way shown above,
-    since it is not as readable as the original statement.  Instead,
-    we use a tactic to introduce the equality within the proof itself.
-    The tactic [(remember t as t')] replaces an object [t] with the
-    identifier [t'] everywhere in the goal and introduces an equality
-    [t' = t] into the context.  It is often combined with [generalize
-    dependent], as illustrated below.
-*)
-
-Lemma typing_weakening_strengthened_1 :  forall (E F G : env) e T,
-  typing_e (G ++ E) e T ->
-  uniq (G ++ F ++ E) ->
-  typing_e (G ++ F ++ E) e T.
-Proof.
-  intros E F G e T H.
-  remember (G ++ E) as E'.
-  generalize dependent G.
-  induction H; intros G0 Eq Uniq; subst.
-  - Case "typing_var". auto.
-  - Case "typing_abs".
-    eapply (typing_e_abs x).
-    (* STILL STUCK! *)
-Admitted.
-
-Print typing_abs.
-
-(** At this point, we are very close. However, there is still one issue. We
-    cannot show that [x] is fresh for the weakened environment [F].
-
-    This is the difficulty with the definition of [typing_e]. As in the local
-    closure judgement, the induction hypotheses is not strong enough in the
-    [abs] case.
-
-    However, this time, we take a slightly different solution. Instead of
-    quantifying over all variables that are fresh for all but a known and
-    fixed set of atoms, we quantify over all variabels that are fresh for all
-    but some, unknown set of atoms.
-
-
-<<
-| typing_abs :
-    forall (L : atoms) (G : env) (T1 : typ) (e : exp) (T2 : typ),
-    (forall x, x `notin` L -> typing ([(x, T1)] ++ G) (e ^ x) T2) ->
-    typing (abs T1 e) (typ_arrow T1 T2) >>
->>
-
-   We call this "cofinite quantification". The advantage of this definition
-   is that it is easier to derive the "exists-fresh" version of the rule
-   [typing_e_abs] as a lemma, than the version we used in [lc_exp].
-   (See below, we prove this lemma after we show substitution.) At the same
-   time, this version of the rule is sufficiently expressive to complete
-   the proof of weakening.
-
-*)
-
-
-(** *** Exercise
-
-    Complete the proof below, using the [typing] relation from [Definitions.v].
-
-    HINTS:
-
-       - The [typing_var] case follows from [binds_weaken], the
-         weakening lemma for the [binds] relation.
-
-       - The [typing_abs] case follows from the induction
-         hypothesis, but the [apply] tactic may be unable to unify
-         things as you might expect.
-
-           -- Recall the [pick fresh and apply] tactic.
-
-           -- In order to apply the induction hypothesis, use
-              [rewrite_env] to reassociate the list operations.
-
-           -- After applying the induction hypothesis, use
-              [simpl_env] to use [uniq_push].
-
-           -- Here, use [auto] to solve facts about finite sets of
-              atoms, since it will simplify the [dom] function behind
-              the scenes.  [fsetdec] does not work with the [dom]
-              function.
-
-       - The [typing_app] case follows directly from the induction
-         hypotheses.
-  *)
-
-Lemma typing_weakening_strengthened :  forall (E F G : env) e T,
-  typing (G ++ E) e T ->
-  uniq (G ++ F ++ E) ->
-  typing (G ++ F ++ E) e T.
-Proof.
-  intros E F G e T H.
-  remember (G ++ E) as E'.
-  generalize dependent G.
-  induction H; intros G0 Eq Uniq; subst.
- (* SOLUTION *)
-  Case "typing_var".
-    apply typing_var.
-      apply Uniq.
-      apply binds_weaken. auto.
-  Case "typing_abs".
-    pick fresh x and apply typing_abs.
-    rewrite_env (((x ~ T1) ++ G0) ++ F ++ E).
-    apply H0.
-      auto.
-      simpl_env. reflexivity.
-      simpl_env. apply uniq_push.
-        apply Uniq.
-        auto.
-  Case "typing_app".
-    eapply typing_app.
-      eapply IHtyping1. reflexivity. apply Uniq.
-      eapply IHtyping2. reflexivity. apply Uniq.
-Qed.
-
-
-(** *** Example
-
-    We can now prove our original statement of weakening.  The only
-    interesting step is the use of the rewrite_env tactic.
-*)
-
-Lemma typing_weakening : forall (E F : env) e T,
-    typing E e T ->
-    uniq (F ++ E) ->
-    typing (F ++ E) e T.
-Proof.
-  intros E F e T H J.
-  rewrite_env (nil ++ F ++ E).
-  apply typing_weakening_strengthened; auto.
-Qed.
-
-
-(*************************************************************************)
-(** * Substitution *)
-(*************************************************************************)
-
-(** Having proved weakening, we can now prove the usual substitution
-    lemma, which we state both in the form we need and in the
-    strengthened form needed to make the proof go through.
-
-<<
-  typing_subst_simple : forall E e u S T z,
-    typing ((z ~ S) ++ E) e T ->
-    typing E u S ->
-    typing E ([z ~> u] e) T
-
-  typing_subst : forall E F e u S T z,
-    typing (F ++ (z ~ S) ++ E) e T ->
-    typing E u S ->
-    typing (F ++ E) ([z ~> u] e) T
->>
-
-    The proof of the strengthened statement proceeds by induction on
-    the given typing derivation for [e].  The most involved case is
-    the one for variables; the others follow from the induction
-    hypotheses.
-*)
-
-
-(** *** Exercise
-
-    Below, we state what needs to be proved in the [typing_var] case
-    of the substitution lemma.  Fill in the proof.
-
-    Proof sketch: The proof proceeds by a case analysis on [(x == z)],
-    i.e., whether the two variables are the same or not.
-
-      - If [(x = z)], then we need to show [(typing (F ++ E) u T)].
-        This follows from the given typing derivation for [u] by
-        weakening and the fact that [T] must equal [S].
-
-      - If [(x <> z)], then we need to show [(typing (F ++ E) x T)].
-        This follows by the typing rule for variables.
-
-    HINTS: Lemmas [binds_mid_eq], [uniq_remove_mid],
-    and [binds_remove_mid] are useful.
-
-  *)
-
-Lemma typing_subst_var_case : forall (E F : env) u S T (z x : atom),
-  binds x T (F ++ (z ~ S) ++ E) ->
-  uniq (F ++ (z ~ S) ++ E) ->
-  typing E u S ->
-  typing (F ++ E) ([z ~> u] (var_f x)) T.
-Proof.
-  intros E F u S T z x H J K.
-  simpl.
- (* SOLUTION *)
-  destruct (x == z).
-  Case "x = z".
-    subst.
-    assert (T = S).
-      eapply binds_mid_eq. apply H. apply J.
-    subst.
-    apply typing_weakening.
-      apply K.
-      eapply uniq_remove_mid. apply J.
-  Case "x <> z".
-    apply typing_var.
-      eapply uniq_remove_mid. apply J.
-      eapply binds_remove_mid. apply H. apply n.
-Qed.
-
-(** *** Note
-
-    The other two cases of the proof of the substitution lemma are
-    relatively straightforward.  However, the case for [typing_abs]
-    needs the fact that the typing relation holds only for
-    locally-closed expressions.
-*)
-
-Lemma typing_to_lc_exp : forall E e T,
-  typing E e T -> lc_exp e.
-Proof.
-  intros E e T H. induction H; eauto.
-Qed.
-
-
-(** *** Exercise
-
-    Complete the proof of the substitution lemma. The proof proceeds
-    by induction on the typing derivation for [e].  The initial steps
-    should use [remember as] and [generalize dependent] in a manner
-    similar to the proof of weakening.
-
-   HINTS:
-      - Use the lemma proved above for the [typing_var] case.
-
-      - The [typing_abs] case follows from the induction hypothesis.
-         -- Use [simpl] to simplify the substitution.
-
-          -- Recall the tactic [pick fresh and apply].
-
-          -- In order to use the induction hypothesis, use
-             [subst_open_var_c] to push the substitution under the
-             opening operation.
-
-          -- Recall the lemma [typing_to_lc_c] and the
-             [rewrite_env] and [simpl_env] tactics.
-
-      - The [typing_app] case follows from the induction hypotheses.
-        Use [simpl] to simplify the substitution.
-*)
-
-Lemma typing_subst : forall (E F : env) e u S T (z : atom),
-  typing (F ++ (z ~ S) ++ E) e T ->
-  typing E u S ->
-  typing (F ++ E) ([z ~> u] e) T.
-Proof.
-(* SOLUTION *)
-  intros E F e u S T z He Hu.
-  remember (F ++ (z ~ S) ++ E) as E'.
-  generalize dependent F.
-  induction He.
-  Case "typing_var".
-    intros F Eq.
-    subst.
-    eapply typing_subst_var_case. apply H0. apply H. apply Hu.
-  Case "typing_abs".
-    intros F Eq.
-    subst.
-    simpl.
-    pick fresh y and apply typing_abs.
-    rewrite subst_exp_open_exp_wrt_exp_var.
-    rewrite_env (((y ~ T1) ++ F) ++ E).
-    apply H0.
-      auto.
-      simpl_env. reflexivity.
-    (* The following subgoals are from [rewrite subst_open_var]. *)
-    auto.
-    eapply typing_to_lc_exp. apply Hu.
-  Case "typing_app".
-    intros F Eq. subst. simpl. eapply typing_app.
-      apply IHHe1. reflexivity.
-      apply IHHe2. reflexivity.
-Qed.
-
-(** *** Exercise
-
-    Complete the proof of the substitution lemma stated in the form we
-    need it.  The proof is similar to that of [typing_weakening].
-
-    HINT: You'll need to use [rewrite_env] to prepend [nil],
-    and [simpl_env] to simplify nil away.
-*)
-
-Lemma typing_subst_simple : forall (E : env) e u S T (z : atom),
-  typing ((z ~ S) ++ E) e T ->
-  typing E u S ->
-  typing E ([z ~> u] e) T.
-Proof.
-(* SOLUTION *)
-  intros E e u S T z H J.
-  rewrite_env (nil ++ E).
-  eapply typing_subst.
-    simpl_env. apply H.
-    apply J.
-Qed.
-
-(*************************************************************************)
-(** * Values and Evaluation *)
-(*************************************************************************)
-
-(** In order to state the preservation lemma, we first need to define
-    values and the small-step evaluation relation.  These inductive
-    relations are straightforward to define.
-
-    Note the hypotheses which ensure that the relations hold only for
-    locally closed terms.  Below, we prove that this is actually the
-    case, since it is not completely obvious from the definitions
-    alone.
-*)
-
-Lemma eval_lc_exp1 : forall e1 e2, eval e1 e2 -> lc_exp e1.
-Proof. induction 1; auto. Qed.
-Lemma eval_lc_exp2 : forall e1 e2, eval e1 e2 -> lc_exp e2.
-Proof. induction 1; auto.
-       - pick fresh x.
-         rewrite (subst_exp_intro x).
-         inversion H0.
-         default_simp.
-         apply subst_exp_lc_exp; auto.
-         fsetdec.
-Qed.
-
-(*************************************************************************)
-(** * Preservation *)
-(*************************************************************************)
-
-(** *** Take-home Exercise
-
-    Complete the proof of preservation.  In this proof, we proceed by
-    induction on the given typing derivation.  The induction
-    hypothesis has already been appropriately generalized by the given
-    proof fragment.
-
-    Proof sketch: By induction on the typing derivation for [e].
-
-      - [typing_var] case: Variables don't step.
-
-      - [typing_abs] case: Abstractions don't step.
-
-      - [typing_app] case: By case analysis on how [e] steps. The
-        [eval_beta] case is interesting, since it follows by the
-        substitution lemma.  The others follow directly from the
-        induction hypotheses.
-*)
-
-  (* HINTS:
-
-       - Use [auto] and [eauto], especially with [;], to solve
-         "uninteresting" subgoals.
-
-       - Use [inversion] to perform case analyses and to rule out
-         impossible cases.
-
-       - In the [eval_beta] subcase of the [typing_app] case:
-
-          -- Use [inversion] on a typing judgement to obtain a
-             hypothesis about when the body of the abstraction is
-             well-typed.
-
-          -- Use [subst_intro] to rewrite the [open] operation into an
-             [open] followed by a [subst].  You'll need to pick a
-             fresh variable first.
-
-  *)
-
-Lemma preservation : forall (E : env) e e' T,
-  typing E e T ->
-  eval e e' ->
-  typing E e' T.
-Proof.
-  intros E e e' T H.
-  generalize dependent e'.
-  induction H; intros e' J.
-(* SOLUTION *)
-  Case "typing_var".
-    inversion J.
-  Case "typing_abs".
-    inversion J.
-  Case "typing_app".
-    inversion J; subst; eauto.
-    SCase "eval_beta".
-      inversion H; subst.
-      pick fresh y.
-      rewrite (subst_exp_intro y); auto.
-      eapply typing_subst_simple; auto.
-Qed.
-
-(*************************************************************************)
-(** * Progress *)
-(*************************************************************************)
-
-(** *** Exercise
-
-    Complete the proof of the progress lemma.  The induction
-    hypothesis has already been appropriately generalized by the given
-    proof fragment.
-
-    Proof sketch: By induction on the typing derivation for [e].
-
-      - [typing_var] case: Can't happen; the empty environment doesn't
-        bind anything.
-
-      - [typing_abs] case: Abstractions are values.
-
-      - [typing_app] case: Applications reduce.  The result follows
-        from an exhaustive case analysis on whether the two components
-        of the application step or are values and the fact that a
-        value must be an abstraction.
-*)
-
-  (* HINTS:
-
-       - Use [auto] and [eauto], especially with [;], to solve
-         "uninteresting" subgoals.
-
-       - Use [inversion] to rule out impossible cases.
-
-       - The lemma [typing_to_lc_c] will be useful for reasoning
-         about local closure.
-
-       - In the [typing_app] case:
-
-          -- Use [destruct] to perform a case analysis on the
-             conclusions of the induction hypotheses.
-
-          -- Use [inversion] on a [value] judgement to determine that
-             the value must be an abstraction.
-  *)
-
-
-
-Lemma progress : forall e T,
-  typing nil e T ->
-  is_value_of_exp e \/ exists e', eval e e'.
-Proof.
-  intros e T H.
-
-  (* It will be useful to have a "non-destructed" form of the given
-     typing derivation, since [induction] takes apart the derivation
-     it is called on. *)
-  assert (typing nil e T); auto.
-
-  (* [remember nil as E] fails here because [nil] takes an implicit
-     argument that Coq is unable to infer.  By prefixing [nil] with
-     [@], we can supply the argument to nil explicitly. *)
-  remember (@nil (atom * typ)) as E.
-
-  induction H; subst.
-
-(* SOLUTION *)
-  - Case "typing_var".
-    inversion H1.
-  - Case "typing_abs".
-    left.
-    simpl. auto.
-  - Case "typing_app".
-    right.
-    destruct IHtyping1 as [V1 | [e1' Eval1]]; auto.
-      + SCase "e1 is a value".
-      destruct IHtyping2 as [V2 | [e2' Eval2]]; auto.
-        SSCase "e2 is a value".
-        destruct e1; inversion V1; subst. exists (open_exp_wrt_exp e1 e2); eauto using typing_to_lc_exp.
-        SSCase "e2 is not a value".
-          exists (app e1 e2'). eauto using typing_to_lc_exp.
-      + SCase "e1 is not a value".
-        exists (app e1' e2).
-        apply eval_app1.
-          eapply typing_to_lc_exp; eauto.
-          assumption.
-Qed.
-
-
-(*************************************************************************)
-(** * Renaming *)
-(*************************************************************************)
-
-(* Substitution and weakening together give us a property we call
-   renaming: (see [typing_rename below] that we can change the name
-   of the variable used to open an expression in a typing
-   derivation. In practice, this means that if a variable is not
-   "fresh enough" during a proof, we can use this lemma to rename it
-   to one with additional freshness constraints.
-
-   Renaming is used below to show the correspondence between the
-   exists-fresh version of the rules with the cofinite version, and
-   also to show that typechecking is decidable.
-*)
-
-(*
-   However, before we prove renaming, we need an auxiliary lemma about
-   typing judgments which says that terms are well-typed only in
-   unique environments.
-*)
-
-Lemma typing_uniq : forall E e T,
-  typing E e T -> uniq E.
-Proof.
-  intros E e T H.
-  induction H; auto.
-  - Case "typing_abs".
-    pick fresh x.
-    assert (uniq ((x ~ T1) ++ G)); auto.
-    inversion H1. auto.
-Qed.
-
-
-(*
-   Demo: the proof of renaming.
-
-   Note that this proof does not proceed by induction: even if we add
-   new typing rules to the language, as long as the weakening and
-   substution properties hold we can use this proof.
-*)
-Lemma typing_rename : forall (x y : atom) E e T1 T2,
-  x `notin` fv_exp e ->
-  y `notin` dom E    ->
-  typing ((x ~ T1) ++ E) (e ^ x) T2 ->
-  typing ((y ~ T1) ++ E) (e ^ y) T2.
-Proof.
-  intros x y E e T1 T2 Fr1 Fr2 H.
-  destruct (x == y).
-  - Case "x = y".
-    subst; eauto.
-  - Case "x <> y".
-    assert (J : uniq ((x ~ T1) ++ E)).
-      eapply typing_uniq; eauto.
-    assert (J' : uniq E).
-      inversion J; eauto.
-    rewrite (@subst_exp_intro x); eauto.
-    rewrite_env (nil ++ (y ~ T1) ++ E).
-    apply typing_subst with (S := T1).
-    simpl_env.
-    + SCase "(open x s) is well-typed".
-      apply typing_weakening_strengthened. eauto. auto.
-    + SCase "y is well-typed".
-      eapply typing_var; eauto.
-Qed.
-
-
-(*************************************************************************)
-(** * Exists-Fresh Definitions *)
-(*************************************************************************)
-
-(* The use of cofinite quantification may make some people worry that we
-   are not formalizing the "right" language. Below, we show that
-   the "exists-fresh" version of the rules is the same as the cofinite
-   version. *)
-
-Lemma typing_abs_exists : forall E e T1 T2 (x : atom),
-      x `notin` fv_exp e ->
-      typing ((x ~ T1) ++ E) (e ^ x) T2 ->
-      typing E (abs T1 e) (typ_arrow T1 T2).
-Proof.
-  intros.
-  apply typing_abs with (L := dom E \u fv_exp e).
-  intros y Fr.
-  apply typing_rename with (x:=x); auto.
-Qed.
-
-
-(*************************************************************************)
-(** * Decidability of Typechecking *)
-(*************************************************************************)
-
-(* Finally, we give another example of a proof that makes use of the
-   renaming lemma. We show that determining whether a program type
-   checks is decidable.
-*)
-
-(** Equality on types is decidable *)
-Lemma eq_typ_dec : forall (T T' : typ),
-  { T = T' } + { T <> T' }.
-Proof.
-  decide equality.
-Qed.
-
-(** Take-home exercise.
-
-    To prove that ill-formed terms cannot be typechecked, we will need an
-    auxiliary lemma that says that each term only has a single type.
-
-    HINT: to prove this lemma you will need to generalize the induction
-    hypothesis for T2 and use the lemma [binds_unique] from [AtomEnv.v].
-*)
-Lemma typing_unique : forall E e T1 T2,
-  typing E e T1 ->
-  typing E e T2 ->
-  T1 = T2.
-Proof.
-(* SOLUTION *)
-  intros E e T1 T2 Typ1 Typ2.
-  generalize dependent T2.
-  induction Typ1; intros T' Typ'; inversion Typ'; subst; eauto.
-  Case "typing_var".
-    eapply binds_unique; eauto.
-  Case "typing_abs".
-    f_equal; eauto.
-    pick fresh x.
-    apply (H0 x); eauto.
-  Case "typing_app".
-    assert (typ_arrow T1 T2 = typ_arrow T3 T') by auto.
-    inversion H; eauto.
-Qed.
-
-
-(* A property P is decidable if we can show the proposition P \/ ~P. *)
-Definition decidable (P : Prop) := (P \/ ~ P).
-
-Lemma typing_decidable : forall E e,
-  lc_exp e -> uniq E -> decidable (exists T, typing E e T).
-Proof.
-  intros E e LC Uniq.
-  generalize dependent E.
-  induction LC; intros E Uniq.
-  - Case "typing_var".
-    destruct (@binds_lookup_dec _ x E) as [[T H] | H].
-      SCase "variable is in environment".
-      left; eauto.
-      SCase "variable not in environment".
-      right.  intros [T J]. inversion J; subst; eauto.
-  - Case "typing_abs".
-    (* To know whether the body typechecks, we must first
-       pick a fresh variable to use the IH (aka HO).
-    *)
-    pick fresh x.
-    destruct (H0 x ((x ~ T) ++ E)) as [[S J] | J]; eauto.
-    SCase "body typeable".
-      left.
-      exists (typ_arrow T S).
-      (* Check (typing_abs L E (abs T e) T S). *)
-      pick fresh z and apply typing_abs.
-      apply typing_rename with (x := x); eauto.
-    SCase "body not typeable".
-      right.
-      intros [S K].
-      inversion K; subst.
-      apply J.
-      exists T2.
-      pick fresh z.
-      apply typing_rename with (x := z); eauto.
-  - Case "typing_app".
-    destruct (IHLC1 E) as [[T H] | H]; eauto.
-    SCase "function typeable".
-      destruct (IHLC2 E) as [[S J] | J]; eauto.
-      SSCase "argument typeable".
-        destruct T.
-          SSSCase "function has typ_base".
-            right.
-            intros [S' J'].
-            inversion J'; subst.
-            assert (K : typ_base = typ_arrow T1 S'); eauto using typing_unique.
-            inversion K.
-          SSSCase "typ_arrow".
-            destruct (eq_typ_dec T1 S).
-              subst. left; eauto.
-              right.
-                intros [S' J'].
-                inversion J'; subst.
-                assert (T3 = S); eauto using typing_unique.
-                assert (typ_arrow T1 T2 = typ_arrow T3 S'); eauto using typing_unique.
-                inversion H1; subst; eauto using typing_unique.
-      SSCase "argument not typeable".
-        right. intros [S' J']. inversion J'; subst; eauto.
-    SCase "function not typeable".
-      right. intros [S' J']. inversion J'; subst; eauto.
-Qed.
-
-(*************************************************************)
-
-(* We also want a property that states that the free variables of well-typed
-   terms are contained within the domain of their typing environments. *)
-Lemma fv_in_dom : forall G e T,
-    typing G e T -> fv_exp e [<=] dom G.
-Proof.
-  intros G e T H.
-  induction H; simpl.
-  - Case "typing_var".
-    apply binds_In in H0.
-    unfold AtomSetImpl.Subset.
-    intros y Iny.
-    assert (y = x). fsetdec. subst.
-    auto.
-  - Case "typing_abs".
-    pick fresh x.
-    assert (Fx : fv_exp (e ^ x) [<=] dom ((x ~ T1) ++ G))
-      by eauto.
-    simpl in Fx.
-    assert (Fy : fv_exp e [<=] fv_exp (e ^ x)) by
-        eapply fv_exp_open_exp_wrt_exp_lower.
-    fsetdec.
-  - fsetdec.
-Qed.
 
 (*************************************************************)
 (* Denotational-interpreter based type soundness proof
@@ -2452,19 +420,317 @@ Proof.
     eapply typing_unload; eauto.
 Qed.
 
+(* ------------------------------------------------------- *)
 
+(* de Bruijn index version *)
+
+Inductive db_val : Set :=
+  | db_closure : typ -> list db_val -> exp -> db_val.
+Definition db_env := list db_val.
+
+
+Fixpoint db_bigstep (n:nat) (e:exp) (rho: db_env) : res db_val :=
+  match n with
+  | 0 => timeout _
+  | S m =>
+    match e with
+    | var_b k => nth k (List.map (val _) rho) (stuck _)
+    | var_f x => stuck _
+    | app e1 e2 =>
+      match db_bigstep m e1 rho with
+      | val _ (db_closure T rho' e1') =>
+        match db_bigstep m e2 rho with
+        | val _ v1 =>
+          db_bigstep m e1' (v1 :: rho')
+        | r => r
+        end
+      | r       => r
+      end
+    | abs T e   => val _ (db_closure T rho e)
+    end
+  end.
+
+Fixpoint close_ctx e (G : env) :=
+  match G with
+  | nil => e
+  | (x,_)::G0 => close_ctx (close_exp_wrt_exp x e) G0
+  end.
+
+
+Fixpoint open_ctx e (G : env) :=
+  match G with
+  | nil => e
+  | (x,_)::G0 => open_ctx (e ^ x) G0
+  end.
+
+Inductive typing_db_val : db_val -> typ -> Prop :=
+ | typing_db_closure : forall T1 T2 G rho e1 L,
+     typing_db_env G rho ->
+     (forall x, x \notin L ->
+           typing ((x ~ T1) ++ G) (open_ctx (e1 ^ x) G) T2) ->
+     typing_db_val (db_closure T1 rho e1) (typ_arrow T1 T2)
+with typing_db_env : env -> db_env -> Prop :=
+ | typing_db_nil  : typing_db_env nil nil
+ | typing_db_cons : forall x v T G rho,
+     typing_db_val v T ->
+     typing_db_env G rho ->
+     x \notin dom G ->
+     typing_db_env ((x ~ T) ++ G) (v :: rho).
+
+Hint Constructors typing_db_val typing_db_env.
+
+(* e has m=length rho dangling bound variables.
+   Let's describe how scoping works in this interpreter.
+ *)
+Inductive scoped_val : db_val -> Prop :=
+  | scoped_closure : forall T rho e,
+      scoped_env rho ->
+      degree_exp_wrt_exp (length rho) (abs T e) ->
+      scoped_val (db_closure T rho e)
+with scoped_env : db_env -> Prop :=
+     | scoped_nil : scoped_env nil
+     | scoped_cons : forall v rho,
+         scoped_val v -> scoped_env rho -> scoped_env (v :: rho).
+Hint Constructors scoped_env scoped_val.
+
+Lemma db_bigstep_scoped : forall n e rho v,
+    scoped_env rho ->
+    degree_exp_wrt_exp (length rho) e ->
+    val _ v = db_bigstep n e rho ->
+    scoped_val v.
+Proof.
+  induction n; intros e rho v SR DE EV; simpl in *.
+  inversion EV.
+  destruct e; inversion DE; subst.
+  - Case "var_b".
+    revert SR EV H1.
+    generalize rho.
+    generalize n0.
+    induction n1; intros; destruct rho0; simpl in *.
+    + inversion EV.
+    + inversion SR. inversion EV. subst. auto.
+    + inversion EV.
+    + inversion SR. subst.
+      eapply IHn1; eauto.
+      apply lt_S_n. auto.
+  - Case "var_f".
+    inversion EV.
+  - Case "abs".
+    inversion EV. eauto.
+  - Case "app".
+    remember (db_bigstep n e1 rho) as r1.
+    remember (db_bigstep n e2 rho) as r2.
+    destruct r1; try solve [inversion EV].
+    destruct d as [T rho' e1'].
+    destruct r2; try solve [inversion EV].
+    assert (SV1: scoped_val (db_closure T rho' e1')) by
+        (eapply (@IHn e1); eauto).
+    assert (SV2: scoped_val d) by (eapply (@IHn e2); eauto).
+    inversion SV1. subst.
+    inversion H5.
+    eapply (@IHn e1' (d :: rho')); eauto.
+Qed.
+
+(* --------------------- *)
+
+Fixpoint db_unload (cv:db_val) : exp :=
+  match cv with
+  | db_closure T rho e =>
+    (fold_left (fun e v => open e (db_unload v)) rho (abs T e))
+  end.
+Definition db_envsubst := fold_left (fun e v => open e (db_unload v)).
+
+Lemma db_unload_is_value : forall v, is_value_of_exp (db_unload v).
+Proof.
+  destruct v. simpl.
+Admitted.
+
+
+(* The next three theorems need to be proven together. To do that we
+   will define a combined induction scheme for the mutual typing
+   judgements typing_rt_val and typing_rt_env.
+ *)
+Scheme scoped_val_ind' := Induction for scoped_val Sort Prop
+ with  scoped_env_ind' := Induction for scoped_env Sort Prop.
+
+Combined Scheme scoped_mutual from scoped_val_ind', scoped_env_ind'.
+
+Lemma db_envsubst_lc_exp_closed : forall rho e,
+    lc_exp e -> db_envsubst rho e = e.
+Proof.
+  induction rho; intros; simpl in *.
+  auto.
+  rewrite open_exp_wrt_exp_lc_exp; auto.
+Qed.
+
+Lemma db_subst_fresh : forall v rho,
+    degree_exp_wrt_exp 0 v -> (db_envsubst rho v) = v.
+Proof.
+  induction rho.
+  simpl. auto.
+  intros. simpl.
+  rewrite open_exp_wrt_exp_lc_exp. auto.
+  apply lc_exp_of_degree. auto.
+Qed.
+
+
+Lemma weaken_degree : forall k n e, degree_exp_wrt_exp n e -> degree_exp_wrt_exp (k + n) e.
+Proof.
+  induction k.
+  auto.
+  intros.
+  simpl.
+Admitted.
+
+Lemma open_first : forall e' e k m,
+    m < k ->
+    degree_exp_wrt_exp 0 e' ->
+    degree_exp_wrt_exp (S k) e ->
+    degree_exp_wrt_exp k (open_exp_wrt_exp_rec m e' e).
+Proof.
+  intros e' e.
+  induction e; simpl.
+  - intros k m LT D.
+    simpl. destruct (lt_eq_lt_dec n m).
+    destruct s; intro h.
+    econstructor. admit.
+    replace k with (k + 0). eapply weaken_degree. auto. admit.
+    intro h.
+    inversion h. subst.
+    econstructor. admit.
+  - intros k m LT D h.
+    econstructor; eauto.
+  - intros k m LT D h.
+    econstructor; eauto.
+    eapply IHe. admit.
+    auto.
+    inversion h.
+    auto.
+  - intros. inversion H1. eauto.
+Admitted.
+
+Lemma db_unload_mutual :
+  (forall v, scoped_val v -> degree_exp_wrt_exp 0 (db_unload v)) /\
+  (forall env, scoped_env env ->
+        Forall (fun x => degree_exp_wrt_exp 0 (db_unload x)) env /\
+        forall e n, degree_exp_wrt_exp (n + (length env)) e ->
+               degree_exp_wrt_exp n (db_envsubst env e)).
+Proof.
+  eapply scoped_mutual; intros.
+  simpl. destruct H. fold db_envsubst. eapply H0. simpl. auto.
+  - split. auto.
+    intros e n H. simpl in *. replace (n + 0) with n in *.  auto. admit.
+  - destruct H0 as [h0 h1]; split; simpl in *.
+    econstructor; eauto.
+    intros e n D.
+    replace (n + S (length rho)) with (S n + length rho) in D.
+    eapply h1.
+    eapply open_first.
+    admit.
+    auto.
+    auto.
+    admit.
+Admitted.
+
+Lemma scoped_val_lc_exp : forall v, scoped_val v -> lc_exp (db_unload v).
+Proof.
+  intros. apply lc_exp_of_degree. eapply db_unload_mutual. auto.
+Qed.
+
+Lemma scoped_env_lc_exp :
+  forall rho, scoped_env rho ->
+         Forall (fun x => lc_exp (db_unload x)) rho.
+Admitted.
+
+
+Lemma db_bigstep_sound : forall n e rho v,
+    db_bigstep n e rho = val _ v ->
+    scoped_env rho ->
+    degree_exp_wrt_exp (length rho) e ->
+    bigstep (db_envsubst rho e) (db_unload v).
+Proof.
+  induction n; intros e rho v EV TR TE; simpl in EV.
+  inversion EV.
+  destruct e.
+  - Case "bvar".
+    revert TR EV TE.
+    generalize rho.
+    generalize n0.
+    induction n1; intros; destruct rho0; simpl in *.
+    + inversion EV.
+    + inversion TR. inversion EV. subst.
+      unfold open. simpl.
+      rewrite db_subst_fresh.
+      econstructor. apply db_unload_is_value.
+      apply scoped_val_lc_exp. auto.
+      admit.
+    + inversion EV.
+    + admit.
+  - Case "fvar". inversion EV.
+  - Case "abs".  inversion EV.
+    econstructor.
+    apply db_unload_is_value.
+    apply scoped_val_lc_exp.
+    econstructor. auto. auto.
+  - Case "app".
+    remember (db_bigstep n e1 rho) as r1.
+    remember (db_bigstep n e2 rho) as r2.
+    destruct r1; try solve [inversion EV].
+    destruct d as [T rho' e1'].
+    destruct r2; try solve [inversion EV].
+Admitted.
+
+Lemma db_bigstep_eval : forall n G e T rho,
+  typing nil (close_ctx e G) T ->
+  typing_db_env G rho ->
+  timeout _ <> db_bigstep n e rho ->
+  exists v, val _ v = db_bigstep n e rho /\ typing_db_val v T.
+Proof.
+  induction n; intros G e T rho TE TR EV; simpl in *.
+  contradiction.
+  destruct e.
+  - Case "var_b".
+    admit.
+  - Case "var_f".
+    admit.
+  - Case "abs".
+    exists (db_closure T0 rho e). split; simpl; eauto.
+    admit.
+  - Case "app".
+    admit.
+
+(*    (* Consider whether e1 evaluates to a value. If it does, apply the IH. *)
+    pose (Ih1 := IHn G e1 (typ_arrow T1 T) rho H2 TR). clearbody Ih1.
+    destruct (db_bigstep n e1 rho); try contradiction;
+    destruct Ih1 as [v1 [EV1 Tv1]]; try solve [intro h; inversion h]; inversion EV1.
+
+    (* By canonical forms, know that v1 must be an abstraction. *)
+    inversion Tv1.  subst.
+
+    (* Consider whether e2 evaluates to a value (and apply the IH if so). *)
+    pose (Ih2 := IHn G e2 T1 rho H4 TR). clearbody Ih2.
+    destruct (db_bigstep n e2 rho); try contradiction;
+    destruct Ih2 as [v2 [EV2 Tv2]]; try solve [intro h; inversion h]; inversion EV2. subst.
+
+    pick fresh x.
+
+    eapply IHn with (G := x ~ T1 ++ G0); eauto.
+
+    pick fresh y. eapply (typing_rename y); eauto.
+    eauto.
+*)
 (* ------------------------------------------------------- *)
 (* Interpreter based big-step semantics *)
 
 Fixpoint rt_bigstep (n:nat) (e:exp) (rho: rt_env) : res rt_val :=
   match n with
-  | 0 => @timeout rt_val
+  | 0 => timeout _
   | S m =>
     match e with
-    | var_b n => @stuck rt_val
+    | var_b n => stuck _
     | var_f x => match (binds_lookup _ x rho) with
                 | inl (exist _ y _) => val _ y
-                | inr _             => @stuck rt_val
+                | inr _             => stuck _
                 end
     | app e1 e2 =>
       match rt_bigstep m e1 rho with
@@ -2481,11 +747,8 @@ Fixpoint rt_bigstep (n:nat) (e:exp) (rho: rt_env) : res rt_val :=
     end
   end.
 
+(* Soundness for definitional interpreter *)
 
-Lemma rt_bigstep_eval : forall n e T,
-  typing nil e T ->
-  @timeout exp <> n_bigstep n e ->
-  exists v, val _ v = n_bigstep n e /\ typing nil v T /\ is_value_of_exp v.
 
 Lemma rt_env_uniq1 : forall G rho,
     typing_rt_env G rho -> uniq G.
@@ -2515,10 +778,67 @@ Proof.
     eauto using rt_env_uniq2.
 Qed.
 
+Lemma notbinds_typing_tr_env : forall G rho x T,
+  typing_rt_env G rho ->
+  binds x T G ->
+  exists v, binds x v rho /\ typing_rt_val v T.
+Proof.
+  induction 1; intros BT.
+  - inversion BT.
+  - simpl in *.
+    apply binds_cons_uniq_1 in BT; eauto using rt_env_uniq1.
+    destruct BT as [[? [? NI1]]| [BT NE1]]. subst.
+    + exists v. split. auto. auto.
+Admitted.
+
+
+Lemma rt_bigstep_eval : forall n G e T rho,
+  typing G e T ->
+  typing_rt_env G rho ->
+  timeout _ <> rt_bigstep n e rho ->
+  exists v, val _ v = rt_bigstep n e rho /\ typing_rt_val v T.
+Proof.
+  induction n; intros G e T rho TE TR EV; simpl in *.
+  contradiction.
+  destruct e; inversion TE; subst.
+  - Case "var_f".
+    destruct (binds_lookup _ x rho) as [[v Pf]|Pf].
+    + (* found *)
+      exists v. split; auto. eapply binds_typing_tr_val; eauto.
+    + (* not found *)
+      admit.
+  - Case "abs".
+    exists (closure T0 rho e). split; simpl; eauto.
+  - Case "app".
+
+
+    (* Consider whether e1 evaluates to a value. If it does, apply the IH. *)
+    pose (Ih1 := IHn G e1 (typ_arrow T1 T) rho H2 TR). clearbody Ih1.
+    destruct (rt_bigstep n e1 rho); try contradiction;
+    destruct Ih1 as [v1 [EV1 Tv1]]; try solve [intro h; inversion h]; inversion EV1.
+
+    (* By canonical forms, know that v1 must be an abstraction. *)
+    inversion Tv1.  subst.
+
+    (* Consider whether e2 evaluates to a value (and apply the IH if so). *)
+    pose (Ih2 := IHn G e2 T1 rho H4 TR). clearbody Ih2.
+    destruct (rt_bigstep n e2 rho); try contradiction;
+    destruct Ih2 as [v2 [EV2 Tv2]]; try solve [intro h; inversion h]; inversion EV2. subst.
+
+    destruct (atom_fresh (dom rho0)) as [x Pf].
+    assert (x `notin` dom G0)
+      by (rewrite same_dom with (rho := rho0); auto).
+
+    eapply IHn with (G := x ~ T1 ++ G0); eauto.
+
+    pick fresh y. eapply (typing_rename y); eauto.
+    eauto.
+Admitted.
+
 Lemma rt_type_soundness : forall n G e T rho v,
   typing G e T ->
   typing_rt_env G rho ->
-  val v = rt_bigstep n e rho ->
+  val _ v = rt_bigstep n e rho ->
   typing_rt_val v T.
 Proof.
   induction n.
@@ -2590,7 +910,7 @@ Admitted.
 
 
 Lemma rt_bigstep_soundness : forall n rho e v,
-    rt_bigstep n e rho = val v ->
+    rt_bigstep n e rho = val _ v ->
     forall G T, typing G e T -> typing_rt_env G rho ->
            bigstep (envsubst rho e) (unload v).
 Proof.
@@ -2616,6 +936,9 @@ Admitted.
 
 (************************************************)
 
+
+
+
 (* Connection between environment & substitution based semantics *)
 
 (* Now let's prove this stepper correct.  Start by showing that it preserves
@@ -2636,7 +959,7 @@ Proof.
   intros.
   inversion H0.
   split.
-  eapply lc_exp.
+Admitted.
 
 Inductive wf_val : rt_val -> Prop :=
 | wf_closure : forall T rho e L,
@@ -2663,7 +986,7 @@ Qed.
 Lemma wf_rt_bigstep : forall n e rho v,
     wf_rho rho   ->
     wf_exp rho e ->
-    val v = rt_bigstep n e rho ->
+    val _ v = rt_bigstep n e rho ->
     wf_val v.
 Proof.
   induction n; intros.
@@ -2696,14 +1019,15 @@ Proof.
          pose (IH2 := IHn e2 rho r H W2 HeqR2). clearbody IH2.
          destruct (atom_fresh (dom rho0)).
          apply (@IHn (e ^ x) ((x,r)::rho0) v); auto.
+         admit.
       -- inversion H1.
       -- inversion H1.
     + inversion H1.
     + inversion H1.
-Qed.
+Admitted.
 
 (* Connection between environment & subst based values: unload and envsubst *)
-
+(*
 Section EnvSubst.
 
 Variable unload    : rt_val -> exp.
@@ -2991,12 +1315,409 @@ Inductive n_exp : Set :=  (*r expressions *)
  | n_abs (x:var) (T:typ) (e:n_exp)
  | n_app (e1:n_exp) (e2:n_exp).
 
-Fixpoint fv_n (e : n_exp) : vars :=
+Fixpoint nom_fv (e : n_exp) : vars :=
   match e with
   | n_var x => {{ x }}
-  | n_abs x T e => AtomSetImpl.remove x (fv_n e)
-  | n_app e1 e2 => fv_n e1 \u fv_n e2
+  | n_abs x T e => AtomSetImpl.remove x (nom_fv e)
+  | n_app e1 e2 => nom_fv e1 \u nom_fv e2
   end.
+
+(* --- translate back to LN rep --- *)
+Fixpoint nom_to_exp (ne : n_exp) : exp :=
+  match ne with
+  | n_var x => var_f x
+  | n_app e1 e2 => app (nom_to_exp e1) (nom_to_exp e2)
+  | n_abs x T e1 => abs T (close_exp_wrt_exp x (nom_to_exp e1))
+end.
+
+Lemma nom_to_exp_lc : forall ne, lc_exp (nom_to_exp ne).
+Proof.
+  induction ne; simpl; auto.
+  eapply lc_abs_exists with (x := x).
+  rewrite open_exp_wrt_exp_close_exp_wrt_exp.
+  auto.
+Qed.
+
+Lemma nom_to_exp_fv : forall ne, nom_fv ne [=] fv_exp (nom_to_exp ne).
+Proof.
+  induction ne; simpl in *.
+  - fsetdec.
+  - rewrite IHne.
+    autorewrite with lngen.
+    fsetdec.
+  - rewrite IHne1. rewrite IHne2.
+    fsetdec.
+Qed.
+
+
+(* Note: this definition does not produce a good induction prinicple.*)
+Inductive nom_val : Set :=
+  | nom_closure : atom -> typ -> nom_env -> n_exp -> nom_val
+with nom_env : Set :=
+  | nom_nil : nom_env
+  | nom_cons : atom -> nom_val -> nom_env -> nom_env.
+
+Scheme nom_val_ind' := Induction for nom_val Sort Prop
+ with  nom_env_ind' := Induction for nom_env Sort Prop.
+Combined Scheme nom_mutual from nom_val_ind', nom_env_ind'.
+
+Fixpoint nom_unload (cv:nom_val) : exp :=
+  match cv with
+  | nom_closure x T rho e =>
+    nom_envsubst rho (nom_to_exp (n_abs x T e))
+  end
+with
+nom_envsubst (ne:nom_env) : exp -> exp :=
+  match ne with
+  | nom_nil => fun e => e
+  | nom_cons x v rho => fun e => nom_envsubst rho (subst_exp (nom_unload v) x e)
+  end.
+
+Fixpoint dom_rho (rho :nom_env) :=
+  match rho with
+  | nom_nil => {}
+  | nom_cons x v rho => {{x}} \u dom_rho rho
+  end.
+
+
+Inductive closed_val : nom_val -> Prop :=
+  | closed_closure : forall x T rho e,
+      closed_env rho ->
+      nom_fv e [<=] {{x}} \u dom_rho rho ->
+      closed_val (nom_closure x T rho e)
+with closed_env : nom_env -> Prop :=
+     | closed_nil : closed_env nom_nil
+     | closed_cons : forall x v rho,
+         closed_val v -> closed_env rho -> closed_env (nom_cons x v rho).
+Hint Constructors closed_env closed_val.
+
+Scheme closed_val_ind' := Induction for closed_val Sort Prop
+ with  closed_env_ind' := Induction for closed_env Sort Prop.
+Combined Scheme closed_nom from closed_val_ind', closed_env_ind'.
+
+Lemma fv_closed_mutual :
+  (forall v, closed_val v -> fv_exp (nom_unload v) [=] {}) /\
+  (forall rho, closed_env rho -> forall e, fv_exp e [<=] dom_rho rho ->
+                                fv_exp (nom_envsubst rho e) [=] {}).
+Proof.
+  eapply closed_nom; intros.
+  + simpl. rewrite H. fsetdec.
+    simpl. autorewrite with lngen.
+    rewrite nom_to_exp_fv in s.
+    fsetdec.
+  + simpl in *. fsetdec.
+  + simpl in *.
+    pose (K := fv_exp_subst_exp_upper (nom_envsubst rho e) (nom_unload v) x). clearbody K.
+Admitted.
+
+Lemma fv_closed :
+  (forall v, closed_val v -> fv_exp (nom_unload v) [=] {}).
+Proof.
+  eapply fv_closed_mutual.
+Qed.
+
+Lemma fv_closed_env :
+  (forall rho, closed_env rho -> forall e, fv_exp e [<=] dom_rho rho ->
+                                fv_exp (nom_envsubst rho e) [=] {}).
+Proof.
+  eapply fv_closed_mutual.
+Qed.
+
+Lemma unload_fresh : forall rho v,
+    closed_val v ->
+    nom_envsubst rho (nom_unload v) = nom_unload v.
+Proof.
+  induction rho. simpl. auto.
+  intros. simpl.
+  rewrite subst_exp_fresh_eq; auto.
+  rewrite fv_closed; auto.
+Qed.
+
+(* Note: maybe replace current metalib defn with this one? *)
+(*
+Program Fixpoint binds_lookup (A:Set) (x:atom) (E:list(atom*A)) :
+  {a : A | binds x a E} + (forall a, ~ binds x a E) :=
+  match E with
+    | nil => inr _
+    | (y,v)::E' => if (x == y) then
+                    inl (exist _ v  _)
+                  else
+                    match binds_lookup _ x E' with
+                      | inl (exist _ v _) => inl (exist _ v _)
+                      | inr _     => inr _
+                    end
+  end.
+Next Obligation.
+intros h. inversion h. inversion H0. subst. contradiction.
+apply n with (a:= a). auto.
+Defined.
+*)
+
+Fixpoint rho_lookup x rho :=
+  match rho with
+  | nom_nil => None
+  | nom_cons y v rho' =>
+    if (x == y) then
+      Some v
+    else
+      rho_lookup x rho'
+  end.
+
+(*
+Lemma binds_lookup : forall A x E,
+    {a : A | binds x a E} + (forall a, ~ binds x a E).
+  Proof with intuition eauto.
+    intros.
+    induction E. right...
+    destruct a as [y v].
+    destruct (eq_dec x y).
+    left. exists v. subst. auto.
+    destruct IHE.
+    destruct s. left...
+    right...
+    inversion H. inversion H0. subst. contradiction.
+    apply n0 with (a:=a). unfold binds. auto.
+  Defined.
+*)
+
+Lemma rho_lookup_closed_val : forall x rho v,
+    closed_env rho ->
+    Some v = rho_lookup x rho ->
+    closed_val v.
+Proof.
+  induction rho; intros; simpl in *.
+  - inversion H0.
+  - inversion H. subst.
+    destruct (x == a).
+    default_simp.
+    eapply IHrho; eauto.
+Qed.
+
+Lemma nom_envsubst_var : forall x rho v,
+    closed_env rho ->
+    Some v = rho_lookup x rho ->
+    nom_envsubst rho (var_f x) = nom_unload v.
+Proof.
+  induction rho.
+  - intros. simpl in *.
+  inversion H0.
+  -  intros. simpl in *.
+     inversion H. subst.
+     destruct (x == a).
+     + inversion H0. subst. clear H0.
+    simpl.
+    rewrite unload_fresh; auto.
+  + eapply IHrho; auto.
+Qed.
+
+Lemma nom_envsubst_abs : forall rho T e,
+ nom_envsubst rho (abs T e) = abs T (nom_envsubst rho e).
+Proof.
+  induction rho; simpl.
+  - auto.
+  - intros.
+    rewrite IHrho.
+    auto.
+Qed.
+
+Lemma nom_envsubst_app : forall rho e1 e2,
+ nom_envsubst rho (app e1 e2) = app (nom_envsubst rho e1) (nom_envsubst rho e2).
+Proof.
+  induction rho; simpl.
+  - auto.
+  - intros.
+    rewrite IHrho.
+    auto.
+Qed.
+
+Lemma nom_unload_is_value : forall v, is_value_of_exp (nom_unload v).
+Proof.
+  destruct v. simpl. rewrite nom_envsubst_abs.
+  simpl. auto.
+Qed.
+
+Inductive Forall_rho (f : nom_val -> Prop) : nom_env -> Prop :=
+| Forall_nom_nil : Forall_rho f nom_nil
+| Forall_nom_cons : forall x a rho, f a -> Forall_rho f rho -> Forall_rho f (nom_cons x a rho).
+
+(*
+Lemma nom_envsubst_lc : forall rho e, Forall_rho  (fun v => lc_exp (nom_unload v)) rho -> lc_exp e -> lc_exp (nom_envsubst rho e).
+Proof.
+  induction rho.
+  intros; simpl; auto.
+  intros; simpl in *.
+  inversion H. subst.
+  eapply IHrho; eauto.
+  eapply subst_exp_lc_exp; eauto.
+Qed.
+*)
+
+Lemma nom_unload_lc_mutual :
+  (forall v, lc_exp (nom_unload v)) /\
+  (forall rho, forall e, lc_exp e -> lc_exp (nom_envsubst rho e)).
+Proof.
+  eapply nom_mutual.
+  - intros. simpl.
+    eapply H.
+    eapply lc_abs_exists with (x:=a).
+    autorewrite with lngen.
+    eapply nom_to_exp_lc.
+  - intros. simpl. auto.
+  - intros; simpl in *.
+    eapply H0; eauto.
+    eapply subst_exp_lc_exp; eauto.
+Qed.
+
+Lemma nom_envsubst_lc : (forall rho, forall e, lc_exp e -> lc_exp (nom_envsubst rho e)).
+  eapply nom_unload_lc_mutual.
+Qed.
+
+Fixpoint nom_bigstep (n:nat) (e:n_exp) (rho: nom_env) : res nom_val :=
+  match n with
+  | 0 => timeout _
+  | S m =>
+    match e with
+    | n_var x =>  match (rho_lookup x rho) with
+                | Some v => val _ v
+                | None   => stuck _
+                end
+    | n_app e1 e2 =>
+      match nom_bigstep m e1 rho with
+      | val _ (nom_closure x T rho' e1') =>
+(*         match AtomSetProperties.In_dec x (dom rho') with
+        | left _ => stuck _
+        | right _ => *)
+            match nom_bigstep m e2 rho with
+            | val _ v1 =>
+              nom_bigstep m e1' (nom_cons x v1 rho')
+            | r => r
+            end
+(*         end *)
+      | r       => r
+      end
+    | n_abs x T e   => val _ (nom_closure x T rho e)
+    end
+  end.
+
+
+
+Lemma nom_closed : forall n rho e v,
+    val _ v = nom_bigstep n e rho ->
+    closed_env rho ->
+    nom_fv e [<=] dom_rho rho ->
+    closed_val v.
+Proof.
+  induction n.
+  intros; simpl in *. inversion H.
+  intros.  destruct e; simpl in *.
+  - Case "var".
+    eapply rho_lookup_closed_val with (x:=x); eauto.
+    destruct (rho_lookup x rho);
+    inversion H;  auto.
+  - Case "abs".
+    inversion H.
+    econstructor; eauto.
+    rewrite <- H1.
+    rewrite <-  AtomSetProperties.add_union_singleton.
+    eapply FSetDecideTestCases.test_Subset_add_remove.
+  - Case "app".
+    remember (nom_bigstep n e1 rho) as r1.
+    remember (nom_bigstep n e2 rho) as r2.
+    destruct r1; try solve [inversion H].
+    assert (C: closed_val n0). eapply IHn; eauto. fsetdec.
+    destruct n0 as [x T rho' e1'].
+    inversion C.
+    destruct r2; try solve [inversion H].
+    assert (closed_val n0). eapply IHn; eauto. fsetdec.
+    eauto.
+Qed.
+
+
+
+Lemma nom_soundness : forall n rho e v,
+    val _ v = nom_bigstep n e rho  ->
+    closed_env rho ->
+    nom_fv e [<=] dom_rho rho ->
+    bigstep (nom_envsubst rho (nom_to_exp e)) (nom_unload v).
+Proof.
+  induction n.
+  intros; simpl in *. inversion H.
+  intros.  destruct e; simpl in *.
+  - Case "var".
+    remember (rho_lookup x rho) as l.
+    destruct l as [[w Pr]| Pr].
+    inversion H. subst. clear H1.
+    erewrite nom_envsubst_var; eauto.
+    econstructor; eauto.
+    eapply nom_unload_is_value.
+    eapply nom_unload_lc_mutual.
+    eapply nom_to_exp_lc.
+    inversion H.
+  - Case "abs".
+    inversion H.
+    subst.
+    simpl.
+    rewrite nom_envsubst_abs.
+    econstructor; eauto.
+    simpl. auto.
+    rewrite <- nom_envsubst_abs.
+    eapply nom_envsubst_lc.
+    eapply lc_abs_exists with (x := x).
+    autorewrite with lngen.
+    eapply nom_to_exp_lc.
+  - Case "app".
+    remember (nom_bigstep n e1 rho) as r1.
+    remember (nom_bigstep n e2 rho) as r2.
+    destruct r1; try solve [inversion H].
+    assert (closed_val n0). eapply nom_closed; eauto. fsetdec.
+    destruct n0 as [x T rho' e1'].
+    inversion H2.
+    destruct r2; try solve [inversion H].
+    assert (closed_val n0). eapply nom_closed; eauto. fsetdec.
+
+    apply IHn in Heqr1; auto; try fsetdec.
+    apply IHn in Heqr2; auto; try fsetdec.
+    simpl in Heqr1.
+    rewrite nom_envsubst_abs in Heqr1.
+
+    apply IHn in H; eauto.
+    simpl in H.
+
+    rewrite nom_envsubst_app.
+    econstructor; eauto.
+    apply nom_unload_is_value.
+
+    rewrite (subst_exp_intro x).
+
+    Focus 2.
+    rewrite fv_closed_env; auto.
+    autorewrite with lngen.
+    admit.
+Admitted.
+
+    pose (IH3 := IHn (nom_cons a v
+
+    fold nom_envsubst.
+    assert (C: closed_val n0). eapply IHn; eauto. fsetdec.
+    destruct n0 as [x T rho' e1'].
+    inversion C.
+
+    assert (closed_val n0). eapply IHn with (e := e2)(rho := rho); eauto. fsetdec.
+    eapply IHn with (e:= e1')(rho:= nom_cons x n0 rho'); eauto.
+Qed.
+
+
+
+(* The next three theorems need to be proven together. To do that we
+   will define a combined induction scheme for the mutual typing
+   judgements typing_rt_val and typing_rt_env.
+ *)
+Scheme typing_val_ind' := Induction for typing_rt_val Sort Prop
+ with  typing_rt_ind' := Induction for typing_rt_env Sort Prop.
+
+Combined Scheme typing_rt from typing_val_ind', typing_rt_ind'.
+
+
 
 
 Definition swap_var (x:var) (y:var) (z:var) : var :=
@@ -3051,8 +1772,8 @@ Inductive aeq : n_exp -> n_exp -> Prop :=
       aeq e1 e1' -> aeq (n_abs x T e1) (n_abs x T e1')
   | aeq_abs_diff : forall x y T e1 e1',
       (forall z,
-          z `notin` fv_n e1' ->
-          z `notin` fv_n e1  ->  (* perhaps unnecessary *)
+          z `notin` nom_fv e1' ->
+          z `notin` nom_fv e1  ->  (* perhaps unnecessary *)
           aeq (swap_n_exp z x e1) (swap_n_exp y x e1')) ->
       aeq (n_abs x T e1) (n_abs y T e1').
 
@@ -3069,7 +1790,7 @@ Inductive named : exp -> n_exp -> Prop :=
 Hint Constructors named.
 
 (* Named terms have the same free variables as LN terms *)
-Lemma named_fv : forall e en, named e en -> fv_exp e [=] fv_n en.
+Lemma named_fv : forall e en, named e en -> fv_exp e [=] nom_fv en.
 Proof.
   induction 1; simpl; auto.
   - fsetdec.
